\documentclass{article}
\usepackage{setspace}

\usepackage{makeidx}         % allows index generation
\usepackage{graphicx}        % standard LaTeX graphics tool
\usepackage{float}
\usepackage[bottom]{footmisc}% places footnotes at page bottom

\usepackage{multirow}
\usepackage{enumitem}
\usepackage{physics}
\usepackage{tensor}
\usepackage{amssymb}
\usepackage{newtxtext}
\usepackage[subscriptcorrection,mtpcal,nofontinfo]{mtpro2}

\begin{document}
\title{Solution to Numerical Relativity: Starting from Scratch}
\maketitle
\tableofcontents

\cleardoublepage

\section{Newton's and Einstein's Gravity}
\subsubsection*{Exercise 1.1}
\begin{enumerate}[label=(\alph*)]
	\item 
\end{enumerate}
\begin{equation*}
	x=y
\end{equation*}

\subsubsection*{Exercise 1.2}
At constant time $t$, constant coordinates $R$ and $\theta$, we have $dt=dR = d\theta = 0$. Therefore, line element becomes
\begin{equation}
	ds^2 = R^2 \sin^2 \frac{\pi}{2} d\phi ^2,
\end{equation}
and we have proper length
\begin{equation}
	C = \int_{0}^{2\pi}dl = \int_0^{2\pi}Rd\phi = 2\pi R.
\end{equation}

\subsubsection*{Exercise 1.3}
\begin{enumerate}[label=(\alph*)]
	\item Given $A^a = (-1, 2, 0, 0)$ and $B^a = (-2, 1, 0, 0)$,
	\begin{equation}
		g_{ab}A^a B^b = -2+2 = 0.
	\end{equation}
	\item Consider only in $t-x$ diagram, $A$ and $B$ will be looks like they do make a angle $\theta = \cos^{-1}\frac{4}{5}\approx 36.87^\circ$.
\end{enumerate}

\subsubsection*{Exercise 1.4}
Since four-velocity defined as
\begin{equation}
	u^a = \frac{dx^a}{d\tau},
\end{equation}
\begin{align}
	u_a u^a &= \frac{dx_a}{d\tau}\frac{dx^a}{d\tau}\\
	&= \frac{g_{ab}dx^adx^b}{d\tau^2}\\
	&= \frac{-ds^2}{d\tau^2}\\
	&= -1.
\end{align}

\section{Foliations of Spacetime: Constraint and Evolution Equations}

\subsubsection*{Exercise 2.1}
From
\begin{equation}
	\mathcal{C}_E = D_i E^i - 4 \pi \rho,
\end{equation}
\begin{equation}
	\partial_t E_i = D_i D^j A_j - D^j D_j A_i - 4 \pi j_i,
\end{equation}
\begin{equation}
	\frac{\partial \rho}{\partial t} + D_i j^i = 0,
\end{equation}
we can get
\begin{align}
	\partial_t \mathcal{C}_E &= D_i \partial_t E^i - 4\pi \frac{\partial \rho}{\partial t}\\
	&= D_i (D^i D^j A_j - D^j D_j A^i - 4\pi j^i) + 4\pi D_i j^i\\
	&= D_i D^i D^j A_j - D_i D^j D_j A^i\\
	&= 0.
\end{align}

\section{Solving the Constraint Equations}

\section{Solving the Evolution Equations}

\section{Numerical Simulations of Black-Hole Binaries}

\end{document}